\documentclass{amsart}
\usepackage{amssymb}
\begin{document}
	\newtheorem{thm}{Theorem}
	\begin{thm}
		$\displaystyle\sum_{i=1}^{n} = \frac{n(n+1)}{2}$, $\forall n \in \mathbf{Z}^+$.
	\end{thm}

	\begin{proof}
	\ \\
	\begin{enumerate}
		\item{for n = 1,}
		\begin{align*}
			& \displaystyle\sum_{i=1}^{1} = 1 \qquad \cdots \cdots \cdots \qquad (1)\\[12pt]
			& \frac{n(n+1)}{2} = \frac{1 \times (1+1)}{2}=1 \qquad \cdots \cdots \cdots \qquad (2)\\[12pt]
			& \because \text{(1) is equal to (2)}\\[12pt]
			& \therefore for\ n = 1,\ the\ equation\ holds.\\[12pt]
		\end{align*}
		
		\item{for n = 2,}
		\begin{align*}
			& \displaystyle\sum_{i=1}^{2} = 1 + 2 = 3 \qquad \cdots \cdots \cdots \qquad (1)\\[12pt]
			& \frac{n(n+1)}{2} = \frac{2 \times (1+2)}{2}=3 \qquad \cdots \cdots \cdots \qquad (2)\\[12pt]
			& \because \text{(1) is equal to (2)}\\[12pt]
			& \therefore for\ n = 2,\ the\ equation\ also\ holds.\\[12pt]
		\end{align*}
		
		\item{Assume for n = k, the equation holds}
		\begin{align*}
			& \displaystyle\sum_{i=1}^{k} = 1 + 2 + 3 + \cdots + k = \frac{k \times (k+1)}{2}\\[12pt]
		\end{align*}
        
        \item{let n = k + 1, such that:}
        \begin{align*}
            target: \displaystyle\sum_{i=1}^{k+1} & = \frac{(k+1)(k+2)}{2} \qquad \cdots \cdots \qquad L.H.S.\\[12pt]
            \displaystyle\sum_{i=1}^{k+1} & = \displaystyle\sum_{i=1}^{k} + (k+1)\\[12pt] 
            & = \frac{k \times (k+1)}{2} + (k+1)\\[12pt] 
            & = \frac{k \times (k+1) + 2(k+1)}{2}\\[12pt]
            & = \frac{(k+2) \times (k+1)}{2} \qquad \cdots \cdots \qquad R.H.S\\[12pt]
        \end{align*}
        \begin{align*}
           & \because\ L.H.S.\ is\ equal\ to\ R.H.S. \\[12pt]
           &  Therefore,\ when\ n = k + 1,\ the\ equation\ holds.\\[12pt] 
        \end{align*}
    \item{According to definitions of Mathematical Induction, the equation holds.}
	\end{enumerate}
	\end{proof}
\end{document} 
