\documentclass {amsart}
\usepackage{amssymb}
\begin {document}
	\newtheorem {thm}{Theorem}
	\begin {thm}
		$\displaystyle\sum_{i=1}^{n} = \frac{n(n+1)}{2}$, $\forall n \in \mathbf{Z}^+$.
	\end {thm}

	\begin {proof}
	\ \\
	\begin {enumerate}
		\item{for n = 1,}
		\begin {align*}
			& \displaystyle\sum_{i=1}^{1} = 1 \qquad \cdots \cdots \cdots \qquad (1)\\[12pt]
			& \frac{n(n+1)}{2} = \frac{1 \times (1+1)}{2}=1 \qquad \cdots \cdots \cdots \qquad (2)\\[12pt]
			& \because \text{(1) is equal to (2)}\\[12pt]
			& \therefore for\ n = 1,\ the\ equation\ holds.\\[12pt]
		\end {align*}
		
		\item{for n = 2,}
		\begin {align*}
			& \displaystyle\sum_{i=1}^{2} = 1 + 2 = 3 \qquad \cdots \cdots \cdots \qquad (1)\\[12pt]
			& \frac{n(n+1)}{2} = \frac{2 \times (1+2)}{2}=3 \qquad \cdots \cdots \cdots \qquad (2)\\[12pt]
			& \because \text{(1) is equal to (2)}\\[12pt]
			& \therefore for\ n = 2,\ the\ equation\ also\ holds.\\[12pt]
		\end {align*}
		
		\item{ Assume for n = k, the equation holds}
		\begin {align*}
			& \displaystyle\sum_{i=1}^{k} = 1 + 2 + 3 + \cdots + k = \frac{k \times (1+k)}{2}\\[12pt]
		\end {align*}
	\end {enumerate}
	\end {proof}
\end {document} 
